eq_types proof

Cm/Pi/Infer.lean
@@ -248,19 +248,20 @@ def infer_eq.eq_types : Expr :=
           infer_eq.no_type))))))))
 
 #eval try_step_n' 1000 (:: apply (:: infer_eq.yes_type (:: infer_nil (:: eq (:: nil nil)))))
-#eval try_step_n' 1000 (:: apply (:: (:: apply (:: infer_eq.eq_types (:: infer_id (:: eq (:: id id))))) (:: infer_nil nil)))
 
-def infer_eq.bind_args : Expr :=
-  (:: both
-    (:: ($? <| (quote infer_eq.assert_op_eq) ·')
-      (quote (quote infer_eq.eq_types))))
+def infer_eq.eq_types_seq : Expr :=
+  infer.assert_seq infer_eq.eq_types
 
-def infer_eq : Expr :=
-  (:: both (:: (quote apply) (:: both (:: (quote Except'.bind) infer_eq.bind_args))))
+#eval try_step_n' 1000 (:: apply (:: infer_eq.eq_types (:: infer_nil (:: eq (:: nil nil)))))
+
+/-def infer_eq : Expr :=
+  (:: both (:: (quote apply) (:: both (:: (quote Except'.bind) infer_eq.bind_args))))-/
 
 namespace infer_test
 
 set_option maxRecDepth 5000
+
+example : try_step_n' 1000 (:: apply (:: infer_eq.eq_types (:: infer_nil (:: eq (:: nil nil))))) = (.ok (:: (symbol "ok") (symbol "Data"))) := rfl
 
 example : try_step_n' 1000 (:: apply (:: (:: apply (:: infer_id (:: infer_nil id))) (:: infer_nil nil))) = (.ok (:: (symbol "ok") (symbol "Data"))) := rfl
 
